Kami/Ex/ProcFourStDec.v
@@ -73,6 +73,7 @@ Section ProcFDE.
                 Expr ty (SyntaxKind (Bit 2)) -> (* opTy *)
                 Expr ty (SyntaxKind (Bit rfIdx)) -> (* dst *)
                 Expr ty (SyntaxKind (Bit addrSize)) -> (* addr *)
+                Expr ty (SyntaxKind (Array Bool dataBytes)) -> (* byteEn *)
                 Expr ty (SyntaxKind (Data dataBytes)) -> (* val1 *)
                 Expr ty (SyntaxKind (Data dataBytes)) -> (* val2 *)
                 Expr ty (SyntaxKind (Data instBytes)) -> (* rawInst *)
@@ -87,6 +88,8 @@ Section ProcFDE.
                         Expr ty (SyntaxKind (Bit rfIdx)))
     (d2eAddr: forall ty, fullType ty (SyntaxKind d2eElt) ->
                          Expr ty (SyntaxKind (Bit addrSize)))
+    (d2eByteEn: forall ty, fullType ty (SyntaxKind d2eElt) ->
+                           Expr ty (SyntaxKind (Array Bool dataBytes)))
     (d2eVal1 d2eVal2: forall ty, fullType ty (SyntaxKind d2eElt) ->
                                  Expr ty (SyntaxKind (Data dataBytes)))
     (d2eRawInst: forall ty, fullType ty (SyntaxKind d2eElt) ->
@@ -128,12 +131,12 @@ Section ProcFDE.
                                      d2eRawInst d2eCurPc e2wPack)
                         ++ epoch
                         ++ PrimFifo.fifo PrimFifo.primPipelineFifoName e2wFifoName e2wElt
-                        ++ (wb dec exec d2eOpType d2eDst d2eAddr d2eVal1 d2eRawInst
+                        ++ (wb dec exec d2eOpType d2eDst d2eAddr d2eByteEn d2eVal1 d2eRawInst
                                d2eCurPc d2eNextPc d2eEpoch e2wDecInst e2wVal))%kami.
 
   Definition p3st := ProcThreeStage.p3st
                        fetch dec exec
-                       d2ePack d2eOpType d2eDst d2eAddr d2eVal1 d2eVal2
+                       d2ePack d2eOpType d2eDst d2eAddr d2eByteEn d2eVal1 d2eVal2
                        d2eRawInst d2eCurPc d2eNextPc d2eEpoch
                        e2wPack e2wDecInst e2wVal init.
 
